MathematicalLogic/FirstOrder/Completeness/Completeness.lean
@@ -18,6 +18,8 @@ theorem Context.Satisfiable.of_consistent : Γ.Consistent → Γ.Satisfiable := 
   apply satisfiable_by_term_model h₂ h₃
   exact henkin_formulas_saturated h₁'
 
+theorem Context.consistent_iff_satisfiable : Γ.Consistent ↔ Γ.Satisfiable := ⟨Satisfiable.of_consistent, Consistent.of_satisfiable⟩
+
 theorem completeness : Γ ⊨ p → Γ ⊢ p := by
   intro h₁
   apply Proof.mp Proof.double_neg2
@@ -33,7 +35,9 @@ theorem completeness : Γ ⊨ p → Γ ⊢ p := by
   apply h₂
   exact Set.mem_insert_of_mem _ h
 
-theorem compactness : Γ ⊨ p → ∃ Δ, Δ ⊆ Γ ∧ Δ.Finite ∧ Δ ⊨ p := by
+theorem provable_iff_entails : Γ ⊢ p ↔ Γ ⊨ p := ⟨soundness, completeness⟩
+
+theorem Entails.compactness : Γ ⊨ p → ∃ Δ, Δ ⊆ Γ ∧ Δ.Finite ∧ Δ ⊨ p := by
   intro h
   apply completeness at h
   apply Proof.compactness at h
@@ -41,8 +45,21 @@ theorem compactness : Γ ⊨ p → ∃ Δ, Δ ⊆ Γ ∧ Δ.Finite ∧ Δ ⊨ p 
   apply soundness at h₃
   exists Δ
 
-theorem Theory.Satisfiable.of_consistent {𝓣 : 𝓛.Theory} :
-  𝓣.Consistent → 𝓣.Satisfiable := by
+theorem Context.Satisfiable.compatcness : Satisfiable.{u} Γ ↔ ∀ Δ ⊆ Γ, Δ.Finite → Satisfiable.{u} Δ := by
+  constructor
+  · intros; apply weaken <;> assumption
+  · intro h
+    rw [←consistent_iff_satisfiable]
+    intro h₁
+    apply Proof.compactness at h₁
+    rcases h₁ with ⟨Δ, h₁, h₂, h₃⟩
+    have h₄ := h Δ h₁ h₂
+    rw [←consistent_iff_satisfiable] at h₄
+    contradiction
+
+variable {𝓣 : 𝓛.Theory}
+
+theorem Theory.Satisfiable.of_consistent : 𝓣.Consistent → 𝓣.Satisfiable := by
   intro h
   apply Context.Satisfiable.of_consistent at h
   rcases h with ⟨𝓢, ρ, h⟩
@@ -51,5 +68,32 @@ theorem Theory.Satisfiable.of_consistent {𝓣 : 𝓛.Theory} :
   rw [Sentence.val_interp_eq]
   apply h
   exists p
+
+theorem Theory.consistent_iff_satisfiable : 𝓣.Consistent ↔ 𝓣.Satisfiable := ⟨Satisfiable.of_consistent, Consistent.of_satisfiable⟩
+
+theorem Theory.complete_iff_elementary_equivalent :
+  𝓣.Complete ↔ ∀ (𝓜 𝓝 : 𝓣.Model), 𝓜 ≃ᴱ (𝓝 : 𝓛.Structure) := by
+  constructor
+  · intro h 𝓜 𝓝 p
+    cases h p with
+    | inl h₁ => simp [soundness' h₁]
+    | inr h₁ => rw [←not_iff_not]; simp [←Sentence.interp_neg, soundness' h₁]
+  · intro h p
+    by_contra h₁; rw [not_or] at h₁; rcases h₁ with ⟨h₁, h₂⟩
+    rw [←Context.Consistent.append'] at h₁
+    apply Context.Satisfiable.of_consistent at h₁
+    rcases h₁ with ⟨𝓜, _, h₁⟩
+    have h₁' := h₁ (~ p).val (Or.inl rfl)
+    rw [←Sentence.val_interp_eq] at h₁'
+    simp [←Context.Consistent.append] at h₂
+    apply Context.Satisfiable.of_consistent at h₂
+    rcases h₂ with ⟨𝓝, _, h₂⟩
+    have h₂' := h₂ p.val (Or.inl rfl)
+    rw [←Sentence.val_interp_eq] at h₂'
+    have h₃ := h ⟨𝓜, by intros p _; rw [Sentence.val_interp_eq]; apply h₁; right; exists p⟩
+      ⟨𝓝, by intros p _; rw [Sentence.val_interp_eq]; apply h₂; right; exists p⟩ p
+    simp at h₃
+    rw [←h₃] at h₂'
+    contradiction
 
 end FirstOrder.Language
